

- $(Y_{i}|X)\sim \text{Bernoulli}(x)$  $\land$   $X\sim \text{uniform}(0,\,1)$
	- where
		- $p_{(Y_{i}|X)}(y_{i}|x)=x^{y_{i}}(1-x)^{1-y_{i}}$
	- let $Y=\sum\limits_{i=1}^{n}Y_{i}\,$,  since $\,(Y_{1},\,\cdots,\,Y_{n}|X)\,$ cond. i.i.d.
		- $p_{(Y|X)}(y|x)=\prod\limits_{i=1}^{n}p_{(Y_{i}|X)}(y_{i}|x)=x^{y}(1-x)^{n-y}$
- $\iff$ 
- $(X|Y)\sim \text{beta}(y+1,\,n-y+1)$
	- where
		- $F_{(X|Y)}(x|y)=\dfrac{1}{B(y+1,\,n-y+1)}B(x;\,y+1,\,n-y+1)$
			- ${\displaystyle\int}_{0}^{x}f_{(X|Y)}(t|y)dt={\displaystyle\int}_{0}^{x}\dfrac{f_{(Y,\,X)}(y,\,t)}{p_{Y}(y)}dt=\dfrac{1}{{\displaystyle\int}_{0}^{1}{f_{(Y,\,X)}(y,\,t)}dt}{\displaystyle\int}_{0}^{x}{f_{(Y,\,X)}(y,\,t)}dt$
			- ${\displaystyle\int}_{0}^{x}{f_{(Y,\,X)}(y,\,t)}dt=B(x;\,y+1,\,n-y+1)$
				- ${\displaystyle\int}_{0}^{x}{p_{(Y|X)}(y|t)\,f_{X}(t)}dt)={\displaystyle\int}_{0}^{x}t^{y}(1-t)^{n-y}dt$

---

- $(Y_{1},\,\cdots,\,Y_{n}|X)$  cond. i.i.d. $\,\,\,\,\not\!\!\!\!\implies$ $(Y_{1},\,\cdots,\,Y_{n})$  i.i.d.
	- (1) $p_{(Y_{1},\,\cdots,\,Y_{n})}(\vec{y})={\displaystyle\int}_{0}^{1}{f_{(Y_{1},\,\cdots,\,Y_{n},\,X)}(y,\,t)}dt=\dfrac{(\sum\limits_{i=1}^{n}y_{i})!\cdot(n-\sum\limits_{i=1}^{n}y_{i})!}{(n+1)!}$
		- { not seperable }
	- (2) $p_{(Y_{n+1}|Y_{1},\,\cdots,\,Y_{n})}(y_{n+1}|\cdots)\neq p_{Y_{n+1}}(y_{n+1})$ { [[Screenshot 2024-01-08 at 6.09.58â€¯PM.png|affected]] }
