
Pf. [product rule] 
		$\displaystyle\lim_{h\to 0}\dfrac{(\frac{f}g)(c+h)-(\frac{f}g)(c)}{h}$ 
		$=\displaystyle\lim_{h\to 0}\dfrac{\frac{f(c+h)}{g(c+h)}-\frac{f(c)}{g(c)}}{h}$
		$=\displaystyle\lim_{h\to 0}\dfrac{{f(c+h)}{g(c)}-{f(c)}{g(c+h)}}{hg(c+h)g(c)}$     (通分)
		$=\displaystyle\lim_{h\to 0}\dfrac{\frac{f(c+h)-f(c)}{h}{g(c)}-{f(c)}\frac{g(c+h)-g(c)}{h}}{g(c+h)g(c)}$  (加一項&減一項)


Pf. [chain rule]
	Let $G(y)=\begin{cases}\dfrac{g(y)-g(f(c))}{y-f(c)},\;\;{\rm if}\;y\neq f(c)\\g'(f(c)),\;\;{\rm if}\;y=f(c)\end{cases}$
	.
	(1) Claim. $G(y)$ is cont. at $f(c)$
		Pf. $G'(f(c))=\displaystyle\lim_{y\to f(c)}\dfrac{g(y)-g(f(c))}{y-f(c)}=g'(f(c))=G(f(c))$
	.
	(2) Claim. $\displaystyle\lim_{h\to 0}\dfrac{(g\circ f)(c+h)-(g\circ f)(c)}{h}=\lim_{h\to0}(G(f(c+h))\cdot\dfrac{f(c+h)-f(c)}{h})$
		case 1. If $f(c+h)=f(c)$, both sides are $0$
		case 2. 
		  If $f(c+h)\neq f(c)$, 
		  $\displaystyle\lim_{h\to 0}\dfrac{(g\circ f)(c+h)-(g\circ f)(c)}{h}=\lim_{h\to 0}(\dfrac{(g\circ f)(c+h)-(g\circ f)(c)}{f(c+h)-f(c)}\cdot\dfrac{f(c+h)-f(c)}{h})$
		  $\displaystyle\lim_{h\to 0}(G(f(c+h))\cdot\dfrac{f(c+h)-f(c)}{h})=G(\lim_{h\to 0}f(c+h))\cdot\lim_{h\to 0}\dfrac{f(c+h)-f(c)}{h}$
		  .
		  therefore
		  $(g\circ f)'(c)=g'(f(c))\cdot f'(c)$
