[ Limit ]

[[2. Thm.#^fadaa3|The Squeeze Thm]]
$\forall\varepsilon>0$ 
$\exists\delta_1>0$ s.t. $0<|x-c|<\delta_1\implies|f(x)-L|<\varepsilon\implies L-\varepsilon < f(x) < L+\varepsilon$
$\exists\delta_2>0$ s.t. $0<|x-c|<\delta_2\implies|h(x)-L|<\varepsilon\implies L-\varepsilon < h(x) < L+\varepsilon$
therefore
$\exists\delta=min(\delta_1,\;\delta_2)>0$
s.t. $0<|x-c|<\delta\implies L-\varepsilon < f(x)\leq g(x)\leq h(x) < L+\varepsilon\implies|g(x)-L|<\varepsilon$
[[2. Thm.#^db3b3a|limit: constant multiple]]
- $\alpha =0 \implies \displaystyle\lim_{x\to c}0=0$
- $\alpha \not =0 \implies$ $\forall\varepsilon>0\;\because\;\exists\delta_1>0$ s.t. $0<|x-c|<\delta_1\implies|f(x)-L|<\varepsilon$
		           $\therefore\;\exists\delta_2=\dfrac{\delta_1}{|\alpha|}$ s.t. $0<|x-c|<\delta_2\implies|\alpha f(x)-\alpha L|<\varepsilon$

[[2. Thm.#^db3b3a|limit: sum]]
$\forall\varepsilon_1>0,\;\exists\delta_1>0$
s.t. $0<|x-c|<\delta_1\implies|f(x)-L|<\varepsilon_1$
$\forall\varepsilon_2>0,\;\exists\delta_2>0$
s.t. $0<|x-c|<\delta_2\implies|g(x)-M|<\varepsilon_2$

$\forall\varepsilon=\varepsilon_1+\varepsilon_2,\;\exists\delta=min(\delta_1,\;\delta_2)$
s.t. $0<|x-c|<\delta\implies|(f(x)+g(x))-(L+M)|=|(f(x)-L)+(g(x)-M)|$     
                      (by Triangular Inequality) 
                      $\leq|(f(x)-L)|+|(g(x)-M)|<\varepsilon_1+\varepsilon_2=\varepsilon$


[ Derivative ]

[[2. Thm.#^656db7|Differentiable => Continuous]]
$\exists$ $\displaystyle\lim_{h\to 0}\dfrac{f(c+h)-f(c)}{h}$ and $\displaystyle\lim_{h\to 0}h=0$
$\implies$ $\displaystyle\lim_{h\to 0}(\dfrac{f(c+h)-f(c)}{h}\cdot h)=0$  by Thm.
$\implies$ $\displaystyle\lim_{h\to 0}({f(c+h)-f(c)})=0$
$\implies$ $\displaystyle\lim_{x\to c}{f(x)}=f(c)$

